src/localdrfra/Stable.v
@@ -1,0 +1,496 @@
+Require Import Omega.
+Require Import Bool.
+Require Import RelationClasses.
+
+From sflib Require Import sflib.
+From Paco Require Import paco.
+
+From PromisingLib Require Import Axioms.
+From PromisingLib Require Import Basic.
+From PromisingLib Require Import DataStructure.
+From PromisingLib Require Import DenseOrder.
+From PromisingLib Require Import Loc.
+From PromisingLib Require Import Language.
+
+Require Import Event.
+Require Import Time.
+Require Import View.
+Require Import Cell.
+Require Import Memory.
+Require Import TView.
+Require Import Local.
+Require Import Thread.
+
+Require Import Trace.
+
+Require Import OrdStep.
+
+Set Implicit Arguments.
+
+
+(* TODO: move *)
+
+Lemma time_le_join_l
+      l r
+      (LE: Time.le r l):
+  Time.join l r = l.
+Proof.
+  unfold Time.join. condtac; auto.
+  apply TimeFacts.antisym; auto.
+Qed.
+
+Lemma time_le_join_r
+      l r
+      (LE: Time.le l r):
+  Time.join l r = r.
+Proof.
+  rewrite Time.join_comm.
+  apply time_le_join_l; auto.
+Qed.
+
+
+Module Stable.
+  Section Stable.
+    Variable L: Loc.t -> bool.
+
+    (* normal *)
+
+    Definition normal_view (view: View.t): Prop :=
+      forall loc (LOC: L loc), view.(View.rlx) loc = view.(View.pln) loc.
+
+    Inductive normal_tview (tview:TView.t): Prop :=
+    | normal_tview_intro
+        (REL: forall loc, normal_view (tview.(TView.rel) loc))
+        (CUR: normal_view tview.(TView.cur))
+        (ACQ: normal_view tview.(TView.acq))
+    .
+
+    Definition normal_memory (mem: Memory.t): Prop :=
+      forall loc from to val released
+        (GET: Memory.get loc to mem = Some (from, Message.concrete val (Some released))),
+        normal_view released.
+
+    Lemma join_normal_view
+          view1 view2
+          (NORMAL1: normal_view view1)
+          (NORMAL2: normal_view view2):
+      normal_view (View.join view1 view2).
+    Proof.
+      ii. unfold normal_view in *.
+      destruct view1, view2. ss.
+      unfold TimeMap.join.
+      rewrite NORMAL1, NORMAL2; ss.
+    Qed.
+
+    Lemma singleton_ur_normal_view loc ts:
+      normal_view (View.singleton_ur loc ts).
+    Proof. ss. Qed.
+
+    Lemma singleton_rw_normal_view
+          loc ts
+          (LOC: ~ L loc):
+      normal_view (View.singleton_rw loc ts).
+    Proof.
+      ii. ss.
+      unfold TimeMap.singleton, LocFun.add, LocFun.init, LocFun.find.
+      condtac; ss. subst. ss.
+    Qed.
+
+    Lemma singleton_ur_if_normal_view
+          b loc ts
+          (LOC: ~ L loc):
+      normal_view (View.singleton_ur_if b loc ts).
+    Proof.
+      unfold View.singleton_ur_if. condtac.
+      - apply singleton_ur_normal_view.
+      - apply singleton_rw_normal_view. ss.
+    Qed.
+
+
+    (* stable *)
+
+    Definition stable_view (mem: Memory.t) (view: View.t): Prop :=
+      forall loc from val released
+        (LOC: L loc)
+        (GET: Memory.get loc (view.(View.rlx) loc) mem =
+              Some (from, Message.concrete val (Some released))),
+        View.le released view.
+
+    Definition stable_timemap (mem: Memory.t) (tm: TimeMap.t): Prop :=
+      stable_view mem (View.mk tm tm).
+
+    Inductive stable_tview (mem: Memory.t) (tview: TView.t): Prop :=
+    | stable_tview_intro
+        (REL: forall loc, stable_view mem (tview.(TView.rel) loc))
+        (CUR: stable_view mem tview.(TView.cur))
+        (ACQ: stable_view mem tview.(TView.acq))
+    .
+
+    Definition stable_memory (mem: Memory.t): Prop :=
+      forall loc from to val released
+        (GET: Memory.get loc to mem = Some (from, Message.concrete val (Some released))),
+        stable_view mem released.
+
+
+    Lemma future_stable_view
+          mem1 mem2 view
+          (CLOSED: Memory.closed_view view mem1)
+          (STABLE: stable_view mem1 view)
+          (MEM_FUTURE: Memory.future mem1 mem2):
+      stable_view mem2 view.
+    Proof.
+      ii. inv CLOSED. specialize (RLX loc). des.
+      exploit Memory.future_get1; try exact RLX; eauto. i. des.
+      rewrite GET0 in *. inv GET. inv MSG_LE. inv RELEASED.
+      exploit STABLE; eauto.
+    Qed.
+
+    Lemma future_stable_tview
+          mem1 mem2 tview
+          (CLOSED: TView.closed tview mem1)
+          (STABLE: stable_tview mem1 tview)
+          (MEM_FUTURE: Memory.future mem1 mem2):
+      stable_tview mem2 tview.
+    Proof.
+      destruct tview. inv CLOSED. inv STABLE. ss.
+      econs; ss; eauto using future_stable_view.
+    Qed.
+
+    Lemma join_stable_view
+          mem view1 view2
+          (STABLE1: stable_view mem view1)
+          (STABLE2: stable_view mem view2):
+      stable_view mem (View.join view1 view2).
+    Proof.
+      ii. unfold stable_view in *.
+      unfold View.join, TimeMap.join in GET. ss.
+      exploit Time.join_cases. i. des.
+      - erewrite x0 in GET.
+        exploit STABLE1; eauto. i.
+        etrans; eauto. apply View.join_l.
+      - erewrite x0 in GET.
+        exploit STABLE2; eauto. i.
+        etrans; eauto. apply View.join_r.
+    Qed.
+
+    Lemma bot_stable_view
+          mem
+          (MEM: Memory.closed mem):
+      stable_view mem View.bot.
+    Proof.
+      ii. inv MEM. rewrite INHABITED in *. inv GET.
+    Qed.
+
+    Lemma singleton_ur_stable_view
+          mem loc ts
+          (MEM: Memory.closed mem)
+          (LOC: ~ L loc):
+      stable_view mem (View.singleton_ur loc ts).
+    Proof.
+      ii. revert GET. ss.
+      unfold TimeMap.singleton, LocFun.add, LocFun.init, LocFun.find.
+      condtac; subst; ss. i.
+      inv MEM. rewrite INHABITED in *. inv GET.
+    Qed.
+
+    Lemma singleton_rw_stable_view
+          mem loc ts
+          (MEM: Memory.closed mem)
+          (LOC: ~ L loc):
+      stable_view mem (View.singleton_rw loc ts).
+    Proof.
+      ii. revert GET. ss.
+      unfold TimeMap.singleton, LocFun.add, LocFun.init, LocFun.find.
+      condtac; subst; ss. i.
+      inv MEM. rewrite INHABITED in *. inv GET.
+    Qed.
+
+    Lemma singleton_ur_if_stable_view
+          mem b loc ts
+          (MEM: Memory.closed mem)
+          (LOC: ~ L loc):
+      stable_view mem (View.singleton_ur_if b loc ts).
+    Proof.
+      unfold View.singleton_ur_if. condtac.
+      - apply singleton_ur_stable_view; ss.
+      - apply singleton_rw_stable_view; ss.
+    Qed.
+
+
+    (* step *)
+
+    Lemma promise_step
+          lc1 mem1 loc from to msg lc2 mem2 kind
+          (WF1: Local.wf lc1 mem1)
+          (MEM1: Memory.closed mem1)
+          (NORMAL_TVIEW1: normal_tview lc1.(Local.tview))
+          (NORMAL_MEM1: normal_memory mem1)
+          (STABLE_TVIEW1: stable_tview mem1 lc1.(Local.tview))
+          (STABLE_MEM1: stable_memory mem1)
+          (MSG: forall val released
+                  (MSG: msg = Message.concrete val (Some released)),
+              normal_view released /\ stable_view mem2 released)
+          (STEP: Local.promise_step lc1 mem1 loc from to msg lc2 mem2 kind):
+      <<NORMAL_TVIEW2: normal_tview lc2.(Local.tview)>> /\
+      <<NORMAL_MEM2: normal_memory mem2>> /\
+      <<STABLE_TVIEW2: stable_tview mem2 lc2.(Local.tview)>> /\
+      <<STABLE_MEM2: stable_memory mem2>>.
+    Proof.
+      inv STEP. inv PROMISE; ss.
+      { (* add *)
+        splits; ss.
+        - ii. revert GET.
+          erewrite Memory.add_o; eauto. condtac; ss; i.
+          + des. subst. inv GET.
+            exploit MSG; eauto. i. des. eauto.
+          + eapply NORMAL_MEM1; eauto.
+        - eapply future_stable_tview; eauto. apply WF1.
+        - ii. revert GET.
+          erewrite Memory.add_o; eauto. condtac; ss; i.
+          + des. subst. inv GET.
+            exploit MSG; eauto. i. des. eauto.
+          + guardH o. inv MEM1. exploit CLOSED0; eauto. i. des.
+            inv MSG_CLOSED. inv CLOSED1. inv CLOSED2.
+            specialize (RLX loc1). des.
+            exploit Memory.future_get1; try exact RLX.
+            { econs 2; eauto. }
+            i. des.
+            rewrite GET1 in *. inv GET0. inv MSG_LE. inv RELEASED.
+            etrans; eauto.
+            eapply STABLE_MEM1; eauto.
+      }
+
+      { (* split *)
+        des. subst.
+        splits; ss.
+        - ii. revert GET.
+          erewrite Memory.split_o; eauto. repeat condtac; ss; i.
+          + des. subst. inv GET.
+            exploit MSG; eauto. i. des. eauto.
+          + guardH o. des. subst. inv GET.
+            exploit Memory.split_get0; try exact MEM. i. des.
+            eapply NORMAL_MEM1; eauto.
+          + eapply NORMAL_MEM1; eauto.
+        - eapply future_stable_tview; eauto. apply WF1.
+        - ii. revert GET.
+          erewrite Memory.split_o; eauto. repeat condtac; ss; i.
+          + des. subst. inv GET.
+            exploit MSG; eauto. i. des. eauto.
+          + guardH o. des. subst. inv GET.
+            exploit Memory.split_get0; try exact MEM. i. des.
+            inv MEM1. exploit CLOSED0; try exact GET1. i. des.
+            inv MSG_CLOSED. inv CLOSED1. inv CLOSED2.
+            specialize (RLX loc1). des.
+            exploit Memory.future_get1; try exact RLX.
+            { econs 2; eauto. }
+            i. des.
+            rewrite GET4 in *. inv GET0. inv MSG_LE. inv RELEASED.
+            etrans; eauto.
+            eapply STABLE_MEM1; eauto.
+          + guardH o. guardH o0.
+            inv MEM1. exploit CLOSED0; eauto. i. des.
+            inv MSG_CLOSED. inv CLOSED1. inv CLOSED2.
+            specialize (RLX loc1). des.
+            exploit Memory.future_get1; try exact RLX.
+            { econs 2; eauto. }
+            i. des.
+            rewrite GET1 in *. inv GET0. inv MSG_LE. inv RELEASED.
+            etrans; eauto.
+            eapply STABLE_MEM1; eauto.
+      }
+
+      { (* lower *)
+        splits; ss.
+        - ii. revert GET.
+          erewrite Memory.lower_o; eauto. condtac; ss; i.
+          + des. subst. inv GET.
+            exploit MSG; eauto. i. des. eauto.
+          + eapply NORMAL_MEM1; eauto.
+        - eapply future_stable_tview; eauto. apply WF1.
+        - ii. revert GET.
+          erewrite Memory.lower_o; eauto. condtac; ss; i.
+          + des. subst. inv GET.
+            exploit MSG; eauto. i. des. eauto.
+          + guardH o. inv MEM1. exploit CLOSED0; eauto. i. des.
+            inv MSG_CLOSED. inv CLOSED1. inv CLOSED2.
+            specialize (RLX loc1). des.
+            exploit Memory.future_get1; try exact RLX.
+            { econs 2; eauto. }
+            i. des.
+            rewrite GET1 in *. inv GET0. inv MSG_LE. inv RELEASED.
+            etrans; eauto.
+            eapply STABLE_MEM1; eauto.
+      }
+
+      { (* cancel *)
+        splits; ss.
+        - ii. revert GET.
+          erewrite Memory.remove_o; eauto. condtac; ss; i.
+          eapply NORMAL_MEM1; eauto.
+        - eapply future_stable_tview; eauto. apply WF1.
+        - ii. revert GET.
+          erewrite Memory.remove_o; eauto. condtac; ss; i.
+          guardH o. inv MEM1. exploit CLOSED0; eauto. i. des.
+          inv MSG_CLOSED. inv CLOSED1. inv CLOSED2.
+          specialize (RLX loc1). des.
+          exploit Memory.future_get1; try exact RLX.
+          { econs 2; eauto. }
+          i. des.
+          rewrite GET1 in *. inv GET0. inv MSG_LE. inv RELEASED.
+          etrans; eauto.
+          eapply STABLE_MEM1; eauto.
+      }
+    Qed.
+
+    Lemma read_step_loc
+          lc1 mem1 loc to val released ord lc2
+          (WF1: Local.wf lc1 mem1)
+          (MEM1: Memory.closed mem1)
+          (NORMAL_TVIEW1: normal_tview lc1.(Local.tview))
+          (NORMAL_MEM1: normal_memory mem1)
+          (STABLE_TVIEW1: stable_tview mem1 lc1.(Local.tview))
+          (STABLE_MEM1: stable_memory mem1)
+          (LOC: L loc)
+          (ORD: Ordering.le Ordering.acqrel ord)
+          (STEP: Local.read_step lc1 mem1 loc to val released ord lc2):
+      <<NORMAL_TVIEW2: normal_tview lc2.(Local.tview)>> /\
+      <<STABLE_TVIEW2: stable_tview mem1 lc2.(Local.tview)>> /\
+      <<LC2: to = lc1.(Local.tview).(TView.cur).(View.rlx) loc -> lc1 = lc2>>.
+    Proof.
+      inv STEP. ss. splits.
+      - inv NORMAL_TVIEW1. econs; ss.
+        + repeat eapply join_normal_view; ss.
+          { destruct ord; ss. }
+          { condtac; ss. destruct released; ss; eauto. }
+        + repeat eapply join_normal_view; ss.
+          { destruct ord; ss. }
+          { condtac; ss. destruct released; ss; eauto. }
+      - inv STABLE_TVIEW1. econs; ss.
+        + unfold View.singleton_ur_if.
+          repeat (condtac; [|destruct ord; ss]). ii.
+          destruct (Loc.eq_dec loc loc0); subst; ss.
+          * unfold TimeMap.join, View.singleton_ur_if,
+            TimeMap.singleton, LocFun.add, LocFun.init, LocFun.find in GET0.
+            revert GET0. condtac; ss. i.
+            rewrite time_le_join_l in GET0; cycle 1.
+            { etrans; [|eapply Time.join_r].
+              inv MEM1. exploit CLOSED; try exact GET. i. des.
+              inv MSG_TS. ss. }
+            rewrite time_le_join_r in GET0; cycle 1.
+            { inv READABLE. auto. }
+            rewrite GET0 in *. inv GET. ss.
+            etrans; [|apply View.join_r]. refl.
+          * unfold TimeMap.join, View.singleton_ur_if,
+            TimeMap.singleton, LocFun.add, LocFun.init, LocFun.find in GET0.
+            revert GET0. condtac; try congr; ss. i.
+            rewrite (@time_le_join_l _ Time.bot) in GET0; try apply Time.bot_spec.
+            exploit Time.join_cases. i. des.
+            { rewrite x0 in GET0.
+              exploit CUR; eauto. i. etrans; eauto.
+              etrans; [|apply View.join_l].
+              etrans; [|apply View.join_l].
+              refl. }
+            { rewrite x0 in GET0. destruct released; ss; cycle 1.
+              { unfold TimeMap.bot in *.
+                inv MEM1. rewrite INHABITED in GET0. ss. }
+              exploit STABLE_MEM1; try exact GET; eauto. i.
+              etrans; eauto.
+              etrans; [|apply View.join_r].
+              refl. }
+        + unfold View.singleton_ur_if.
+          repeat (condtac; [|destruct ord; ss]). ii.
+          destruct (Loc.eq_dec loc loc0); subst; ss.
+          * unfold TimeMap.join, View.singleton_ur_if,
+            TimeMap.singleton, LocFun.add, LocFun.init, LocFun.find in GET0.
+            revert GET0. condtac; ss. i.
+            rewrite Time.join_assoc in GET0.
+            rewrite (@time_le_join_l to) in GET0; cycle 1.
+            { inv MEM1. exploit CLOSED; try exact GET. i. des.
+              inv MSG_TS. ss. }
+            exploit Time.join_cases. i. des.
+            { rewrite x0 in GET0.
+              exploit ACQ; eauto. i. etrans; eauto.
+              etrans; [|apply View.join_l].
+              etrans; [|apply View.join_l].
+              refl. }
+            { rewrite x0 in GET0. rewrite GET0 in *. inv GET. ss.
+              etrans; [|apply View.join_r]. 
+              refl. }
+          * unfold TimeMap.join, View.singleton_ur_if,
+            TimeMap.singleton, LocFun.add, LocFun.init, LocFun.find in GET0.
+            revert GET0. condtac; try congr; ss. i.
+            rewrite (@time_le_join_l _ Time.bot) in GET0; try apply Time.bot_spec.
+            exploit Time.join_cases. i. des.
+            { rewrite x0 in GET0.
+              exploit ACQ; eauto. i. etrans; eauto.
+              etrans; [|apply View.join_l].
+              etrans; [|apply View.join_l].
+              refl. }
+            { rewrite x0 in GET0. destruct released; ss; cycle 1.
+              { unfold TimeMap.bot in *.
+                inv MEM1. rewrite INHABITED in GET0. ss. }
+              exploit STABLE_MEM1; try exact GET; eauto. i.
+              etrans; eauto.
+              etrans; [|apply View.join_r].
+              refl. }
+      - i. subst. destruct lc1. f_equal; ss.
+        unfold TView.read_tview. condtac; ss. condtac; [|destruct ord]; ss.
+        destruct tview; ss. f_equal; ss.
+        + repeat rewrite View.le_join_l; ss.
+          * eapply View.singleton_ur_spec; try apply WF1.
+            inv NORMAL_TVIEW1. rewrite CUR; ss. refl.
+          * destruct released; try apply View.bot_spec. ss.
+            inv STABLE_TVIEW1. eauto.
+          * eapply View.singleton_ur_spec; try apply WF1.
+            inv NORMAL_TVIEW1. rewrite CUR; ss. refl.
+        + repeat rewrite View.le_join_l; ss.
+          * inv WF1. ss. inv TVIEW_WF. ss. etrans; eauto.
+            eapply View.singleton_ur_spec; ss.
+            inv NORMAL_TVIEW1. rewrite CUR0; ss. refl.
+          * inv WF1. ss. inv TVIEW_WF. ss. etrans; eauto.
+            destruct released; try apply View.bot_spec. ss.
+            inv STABLE_TVIEW1. eauto.
+          * inv WF1. ss. inv TVIEW_WF. ss. etrans; eauto.
+            eapply View.singleton_ur_spec; ss.
+            inv NORMAL_TVIEW1. rewrite CUR0; ss. refl.
+    Qed.
+
+    Lemma read_step_other
+          lc1 mem1 loc to val released ord lc2
+          (WF1: Local.wf lc1 mem1)
+          (MEM1: Memory.closed mem1)
+          (NORMAL_TVIEW1: normal_tview lc1.(Local.tview))
+          (NORMAL_MEM1: normal_memory mem1)
+          (STABLE_TVIEW1: stable_tview mem1 lc1.(Local.tview))
+          (STABLE_MEM1: stable_memory mem1)
+          (LOC: ~ L loc)
+          (STEP: Local.read_step lc1 mem1 loc to val released ord lc2):
+      <<NORMAL_TVIEW2: normal_tview lc2.(Local.tview)>> /\
+      <<STABLE_TVIEW2: stable_tview mem1 lc2.(Local.tview)>>.
+    Proof.
+      inv STEP. ss. splits.
+      - inv NORMAL_TVIEW1. econs; ss.
+        + repeat apply join_normal_view; ss.
+          * apply singleton_ur_if_normal_view. ss.
+          * condtac; ss. destruct released; ss. eauto.
+        + repeat apply join_normal_view; ss.
+          * apply singleton_ur_if_normal_view. ss.
+          * condtac; ss. destruct released; ss. eauto.
+      - inv STABLE_TVIEW1. econs; ss.
+        + repeat apply join_stable_view; ss.
+          * apply singleton_ur_if_stable_view; ss.
+          * condtac; ss.
+            { destruct released; ss.
+              - eapply STABLE_MEM1; eauto.
+              - apply bot_stable_view; ss. }
+            { apply bot_stable_view; ss. }
+        + repeat apply join_stable_view; ss.
+          * apply singleton_ur_if_stable_view; ss.
+          * condtac; ss.
+            { destruct released; ss.
+              - eapply STABLE_MEM1; eauto.
+              - apply bot_stable_view; ss. }
+            { apply bot_stable_view; ss. }
+    Qed.
+  End Stable.
+End Stable.
